crates/minocrab-zkir/lean/MinocrabZkir.lean
@@ -3,4 +3,6 @@ import MinocrabZkir.Print
 import MinocrabZkir.Parse
 import MinocrabZkir.Dataflow
 import MinocrabZkir.Semantics
+import MinocrabZkir.Constraint
+import MinocrabZkir.Completeness
 import MinocrabZkir.Smoke
